backend/RTL.v
@@ -262,12 +262,11 @@ Inductive step: state -> trace -> state -> Prop :=
       step (State s f sp pc rs m)
         E0 (State s f sp pc' rs m)
   | exec_Ireturn:
-      forall s f stk pc rs m or m' m'',
+      forall s f stk pc rs m or m',
       (fn_code f)!pc = Some(Ireturn or) ->
       Mem.free_frame m = Some m' ->
-      Mem.free m' stk 0 f.(fn_stacksize) = Some m'' ->
       step (State s f (Vptr stk Ptrofs.zero) pc rs m)
-        E0 (Returnstate s (regmap_optget or Vundef rs) m'')
+        E0 (Returnstate s (regmap_optget or Vundef rs) m')
   | exec_function_internal:
       forall s f args m m' m'' stk,
       Mem.alloc_frame m = m' ->
