backend/Unusedglobproof.v
@@ -686,14 +686,14 @@ Inductive match_stacks (j: meminj):
       Mem.sup_include (Genv.genv_sup tge) tbound ->
       match_stacks j nil nil bound tbound
   | match_stacks_cons: forall res f sps sp pc rs s tsps tsp trs ts bound tbound
-         (SPS: sp = fresh_block true sps)
-         (TSPS: tsp = fresh_block true tsps)
+         (SPS: sp = fresh_block sps)
+         (TSPS: tsp = fresh_block tsps)
          (STACKS: match_stacks j s ts sps tsps)
          (KEPT: forall id, ref_function f id -> kept id)
          (SPINJ: j sp = Some(tsp, 0))
          (REGINJ: regset_inject j rs trs)
-         (BELOW: Mem.sup_include (sup_incr true sps) bound)
-         (TBELOW: Mem.sup_include (sup_incr true tsps) tbound),
+         (BELOW: Mem.sup_include (sup_incr sps) bound)
+         (TBELOW: Mem.sup_include (sup_incr tsps) tbound),
       match_stacks j (Stackframe res f (Vptr sp Ptrofs.zero) pc rs :: s)
                      (Stackframe res f (Vptr tsp Ptrofs.zero) pc trs :: ts)
                      bound tbound.
@@ -758,8 +758,8 @@ Qed.
 
 Inductive match_states: state -> state -> Prop :=
   | match_states_regular: forall s f sp sps pc rs m ts tsp tsps trs tm j
-         (SPS: sp = fresh_block true sps)
-         (TSPS: tsp = fresh_block true tsps)
+         (SPS: sp = fresh_block sps)
+         (TSPS: tsp = fresh_block tsps)
          (STACKS: match_stacks j s ts sps tsps)
          (KEPT: forall id, ref_function f id -> kept id)
          (SPINJ: j sp = Some(tsp, 0))
@@ -901,9 +901,9 @@ Proof.
 
 - (* op *)
   assert (A: exists tv,
-               eval_operation tge (Vptr (fresh_block true tsps) Ptrofs.zero) op trs##args tm = Some tv
+               eval_operation tge (Vptr (fresh_block tsps) Ptrofs.zero) op trs##args tm = Some tv
             /\ Val.inject j v tv).
-  { apply eval_operation_inj with (ge1 := ge) (m1 := m) (sp1 := Vptr (fresh_block true sps) Ptrofs.zero) (vl1 := rs##args).
+  { apply eval_operation_inj with (ge1 := ge) (m1 := m) (sp1 := Vptr (fresh_block sps) Ptrofs.zero) (vl1 := rs##args).
     intros; eapply Mem.valid_pointer_inject_val; eauto.
     intros; eapply Mem.weak_valid_pointer_inject_val; eauto.
     intros; eapply Mem.weak_valid_pointer_inject_no_overflow; eauto.
@@ -919,9 +919,9 @@ Proof.
 
 - (* load *)
   assert (A: exists ta,
-               eval_addressing tge (Vptr (fresh_block true tsps) Ptrofs.zero) addr trs##args = Some ta
+               eval_addressing tge (Vptr (fresh_block tsps) Ptrofs.zero) addr trs##args = Some ta
             /\ Val.inject j a ta).
-  { apply eval_addressing_inj with (ge1 := ge) (sp1 := Vptr (fresh_block true sps) Ptrofs.zero) (vl1 := rs##args).
+  { apply eval_addressing_inj with (ge1 := ge) (sp1 := Vptr (fresh_block sps) Ptrofs.zero) (vl1 := rs##args).
     intros. apply symbol_address_inject. eapply match_stacks_preserves_globals; eauto.
     apply KEPT. red. exists pc, (Iload chunk addr args dst pc'); auto.
     econstructor; eauto.
@@ -934,9 +934,9 @@ Proof.
 
 - (* store *)
   assert (A: exists ta,
-               eval_addressing tge (Vptr (fresh_block true tsps) Ptrofs.zero) addr trs##args = Some ta
+               eval_addressing tge (Vptr (fresh_block tsps) Ptrofs.zero) addr trs##args = Some ta
             /\ Val.inject j a ta).
-  { apply eval_addressing_inj with (ge1 := ge) (sp1 := Vptr (fresh_block true sps) Ptrofs.zero) (vl1 := rs##args).
+  { apply eval_addressing_inj with (ge1 := ge) (sp1 := Vptr (fresh_block sps) Ptrofs.zero) (vl1 := rs##args).
     intros. apply symbol_address_inject. eapply match_stacks_preserves_globals; eauto.
     apply KEPT. red. exists pc, (Istore chunk addr args src pc'); auto.
     econstructor; eauto.
@@ -1009,13 +1009,17 @@ Proof.
   econstructor; eauto.
 
 - (* return *)
-  exploit Mem.free_parallel_inject; eauto. rewrite ! Z.add_0_r. intros (tm' & C & D).
+  Search inject_incr.
+  assert (exists j' tm', Mem.free_frame tm = Some tm' /\ Mem.inject j' m' tm').
+  admit.
+  destruct H1 as (j'&tm'&FREE&INJ').
   econstructor; split.
   eapply exec_Ireturn; eauto.
   econstructor; eauto.
-  apply match_stacks_bound with sps tsps; auto.
+  admit.
+(*  apply match_stacks_bound with sps tsps; auto.
   erewrite Mem.support_free; eauto.
-  erewrite Mem.support_free; eauto.
+  erewrite Mem.support_free; eauto. *)
   destruct or; simpl; auto.
 
 - (* internal function *)
